edited some fomatting

SeqOfSeq.dfy
@@ -6,34 +6,34 @@ module SeqOfSeq {
 
   /*concatenates a sequence of sequences into a single sequence. 
   Works by adding elements in order from first to last */
-  function method seq_concat<T>(seqs: seq<seq<T>>): seq<T>
-  decreases |seqs|
+  function method seq_concat<T>(s: seq<seq<T>>): seq<T>
+  decreases |s|
   {
-    if |seqs| == 0 then []
-    else seqs[0] + seq_concat(seqs[1..])
+    if |s| == 0 then []
+    else s[0] + seq_concat(s[1..])
   }
 
   // turns a sequence of sequences into a single sequence and returns the result
-  function method {:opaque} concat_seq<A>(a: seq<seq<A>>): seq<A>
+  function method {:opaque} concat_seq<T>(s: seq<seq<T>>): seq<T>
   {
-    if |a| == 0 then [] else concat_seq(drop_last(a)) + last(a)
+    if |s| == 0 then [] else concat_seq(drop_last(s)) + last(s)
   }
 
     /* concatenating two sequences of sequences is equivalent to concatenating
   each sequence of sequences seperately, and then concatenating the two resulting 
   sequences together */
-  lemma lemma_seq_concat_adds<T>(A:seq<seq<T>>, B:seq<seq<T>>)
-    ensures seq_concat(A + B) == seq_concat(A) + seq_concat(B)
+  lemma lemma_seq_concat_adds<T>(a: seq<seq<T>>, b: seq<seq<T>>)
+    ensures seq_concat(a + b) == seq_concat(a) + seq_concat(b)
   {
-    if |A| == 0 {
-      assert A+B == B;
+    if |a| == 0 {
+      assert a + b == b;
     } else {
       calc == {
-        seq_concat(A + B);
-          { assert (A + B)[0] == A[0];  assert (A + B)[1..] == A[1..] + B; }
-        A[0] + seq_concat(A[1..] + B);
-        A[0] + seq_concat(A[1..]) + seq_concat(B);
-        seq_concat(A) + seq_concat(B);
+        seq_concat(a + b);
+          { assert (a + b)[0] == a[0];  assert (a + b)[1..] == a[1..] + b; }
+        a[0] + seq_concat(a[1..] + b);
+        a[0] + seq_concat(a[1..]) + seq_concat(b);
+        seq_concat(a) + seq_concat(b);
       }
     }
   }
@@ -75,11 +75,11 @@ module SeqOfSeq {
 
   /* concatenates the sequence of sequences into a single sequence. 
   works by adding elements from last to first */
-  function method seq_concat_reverse<T>(seqs: seq<seq<T>>): seq<T>
-  decreases |seqs|
+  function method seq_concat_reverse<T>(s: seq<seq<T>>): seq<T>
+  decreases |s|
   {
-    if |seqs| == 0 then []
-    else seq_concat_reverse(drop_last(seqs)) + last(seqs)
+    if |s| == 0 then []
+    else seq_concat_reverse(drop_last(s)) + last(s)
   }
 
   /* concatenating two reversed sequences of sequences is the same as reversing two 
@@ -103,47 +103,47 @@ module SeqOfSeq {
 
   /* both methods of concatenating sequence (starting from front v. starting from back)
   result in the same sequence */
-  lemma lemma_seq_concat_and_seq_concat_reverse_are_equivalent<T>(seqs: seq<seq<T>>)
-    ensures seq_concat(seqs) == seq_concat_reverse(seqs)
+  lemma lemma_seq_concat_and_seq_concat_reverse_are_equivalent<T>(s: seq<seq<T>>)
+    ensures seq_concat(s) == seq_concat_reverse(s)
   {
-    if |seqs| == 0 {
+    if |s| == 0 {
     } else {
       calc == {
-        seq_concat_reverse(seqs);
-        seq_concat_reverse(drop_last(seqs)) + last(seqs);
-          { lemma_seq_concat_and_seq_concat_reverse_are_equivalent(drop_last(seqs)); }
-        seq_concat(drop_last(seqs)) + last(seqs);
-        seq_concat(drop_last(seqs)) + seq_concat([last(seqs)]);
-          { lemma_seq_concat_adds(drop_last(seqs), [last(seqs)]); 
-        assert seqs == drop_last(seqs) + [last(seqs)]; }
-        seq_concat(seqs);
+        seq_concat_reverse(s);
+        seq_concat_reverse(drop_last(s)) + last(s);
+          { lemma_seq_concat_and_seq_concat_reverse_are_equivalent(drop_last(s)); }
+        seq_concat(drop_last(s)) + last(s);
+        seq_concat(drop_last(s)) + seq_concat([last(s)]);
+          { lemma_seq_concat_adds(drop_last(s), [last(s)]); 
+        assert s == drop_last(s) + [last(s)]; }
+        seq_concat(s);
       }
     }
   }
 
   /* the concatenated sequence's length is greater than or equal to 
   each individual inner sequence's length */
-  lemma lemma_concat_seq_length_ge_single_element_length<A>(a: seq<seq<A>>, i: int)
-  requires 0 <= i < |a|
-  ensures |concat_seq(a)| >= |a[i]|
+  lemma lemma_concat_seq_length_ge_single_element_length<T>(s: seq<seq<T>>, i: int)
+  requires 0 <= i < |s|
+  ensures |concat_seq(s)| >= |s[i]|
   {
     reveal_concat_seq();
-    if i < |a| - 1 {
-      lemma_concat_seq_length_ge_single_element_length(a[..|a|-1], i);
+    if i < |s| - 1 {
+      lemma_concat_seq_length_ge_single_element_length(s[..|s|-1], i);
     }
   }
 
   /* the length of concatenating sequence in a sequence together will be no longer 
   than the length of the original sequence of sequences multiplied by the length of 
   the longest sequence */
-  lemma lemma_concat_seq_length_le_mul<A>(a: seq<seq<A>>, t: int)
-  requires forall i | 0 <= i < |a| :: |a[i]| <= t
-  ensures |concat_seq(a)| <= |a| * t
+  lemma lemma_concat_seq_length_le_mul<T>(s: seq<seq<T>>, j: int)
+  requires forall i | 0 <= i < |s| :: |s[i]| <= j
+  ensures |concat_seq(s)| <= |s| * j
   {
     reveal_concat_seq();
-    if |a| == 0 {
+    if |s| == 0 {
     } else {
-      lemma_concat_seq_length_le_mul(a[..|a|-1], t);
+      lemma_concat_seq_length_le_mul(s[..|s|-1], j);
     }
   }
 
